test.lean
@@ -1,0 +1,8 @@
+import Complexity.Complexity.Definitions
+
+example : inOPoly (fun n => n) := by
+  unfold inOPoly inO
+  use 1
+  use 0
+  intro n hn
+  sorry
